\[
\int \frac{2 e^{2 x}-e^x}{\sqrt{3 e^{2 x}-6 e^x-1}} d x \\
\]

\[
\begin{aligned}
& \int \frac{2 e^{2 x}-e^x}{\sqrt{3 e^{2 x}-6 e^x-1}} d x = \int \frac{(2 e^x-1) e^x}{\sqrt{3(e^{2 x}-2 e^x-\frac{1}{3})}} d x \\
& = \int \frac{(2 e^x-1) e^x}{\sqrt{3} \sqrt{e^{2 x}-2 e^x-\frac{1}{3}}} d x \\
& = \frac{1}{\sqrt{3}} \int \frac{(2 e^x-1) e^x}{\sqrt{e^{2 x}-2 e^x-\frac{1}{3}}} d x \\
\end{aligned}\\
\]

Let $u=e^x$ and $du=e^x dx$. Then:

\[
\begin{aligned}
& \frac{1}{\sqrt{3}} \int \frac{(2 e^x-1) e^x}{\sqrt{e^{2 x}-2 e^x-\frac{1}{3}}} d x \\
& = \frac{1}{\sqrt{3}} \int \frac{(2 u-1)}{\sqrt{u^2-2 u-\frac{1}{3}}} du \\
& = \frac{2}{3} \int \frac{\sec \theta \tan \theta}{\sqrt{\tan^2 \theta}} d \theta \\
& = \frac{2}{3} \int \sec \theta d \theta \\
& = \frac{2}{3} \ln \left|\sec \theta + \tan \theta\right| \\
& = \frac{2}{3} \ln \left|\sqrt{\frac{3 u^2-6u-1}{3}}+u-1\right| \\
& = \frac{1}{\sqrt{3}} \ln \left(\frac{\sqrt{3}}{2}\left(e^x-1+\frac{1}{\sqrt{3}} \sqrt{3 e^{2 x}-6 e^x-1}\right)\right) \\
\end{aligned}
\]
