$$\int \frac{2e^{2x}-e^x}{\sqrt{3e^{2x}-6e^x-1}},dx$$

\begin{align*}
&\int \frac{2e^{2x}-e^x}{\sqrt{3e^{2x}-6e^x-1}},dx = \int \frac{(2e^x-1)e^x}{\sqrt{3(e^{2x}-2e^x-\frac{1}{3})}},dx\
&= \int \frac{(2e^x-1)e^x}{\sqrt{3}\sqrt{e^{2x}-2e^x-\frac{1}{3}}},dx\
&= \frac{1}{\sqrt{3}} \int \frac{(2e^x-1)e^x}{\sqrt{e^{2x}-2e^x-\frac{1}{3}}},dx
\end{align*}

Let $u=e^x$ and $du=e^x,dx$. Then:

\begin{align*}
&\frac{1}{\sqrt{3}} \int \frac{(2e^x-1)e^x}{\sqrt{e^{2x}-2e^x-\frac{1}{3}}},dx\
&= \frac{1}{\sqrt{3}} \int \frac{(2u-1)}{\sqrt{u^2-2u-\frac{1}{3}}},du\
&= \frac{2}{3} \int \frac{\sec\theta\tan\theta}{\sqrt{\tan^2\theta}},d\theta\
&= \frac{2}{3} \int \sec\theta,d\theta\
&= \frac{2}{3} \ln\left|\sec\theta+\tan\theta\right|\
&= \frac{2}{3} \ln\left|\sqrt{\frac{3u^2-6u-1}{3}}+u-1\right|\
&= \frac{1}{\sqrt{3}} \ln\left(\frac{\sqrt{3}}{2}\left(e^x-1+\frac{1}{\sqrt{3}}\sqrt{3e^{2x}-6e^x-1}\right)\right)\
\end{align*}
